Downgrading Security Specification (#1844)
This is a candidate specification of a security condition that does permit downgrades and ensures that the only way around the information flow labels is through these downgrades. There is just a partial specification of the model that supports downgrades that includes just one call so that the proof effort can focus on the proof structure and the model can be scaled up later.

experimental/ni_coq/vfiles/LowEquivalences.v
@@ -73,6 +73,7 @@ Definition low_proj {A: Type} ell ( labeled_thing: @labeled A) :=
 Definition node_low_proj := @low_proj node.
 Definition chan_low_proj := @low_proj channel.
 Definition event_low_proj := @low_proj event.
+Definition down_low_proj := @low_proj down_event.
 
 Definition node_state_low_proj (ell: level)(ns: node_state): node_state :=
     fun id => low_proj ell (ns id).
@@ -96,6 +97,7 @@ Definition low_eq {A: Type} ell (x: @labeled A) (y: @labeled A) :=
 Definition node_low_eq := @low_eq node.
 Definition chan_low_eq := @low_eq channel.
 Definition event_low_eq := @low_eq event.
+Definition down_low_eq := @low_eq down_event.
 Definition node_state_low_eq := fun ell ns1 ns2 =>
     forall nid, (node_state_low_proj ell ns1) nid = (node_state_low_proj ell ns2) nid.
 Definition chan_state_low_eq := fun ell cs1 cs2 =>
@@ -105,98 +107,3 @@ Definition state_low_eq := fun ell s1 s2 =>
         (state_low_proj ell s2).(nodes) nid) /\
     (forall han, (state_low_proj ell s1).(chans) han=
         (state_low_proj ell s2).(chans) han ).
-
-(*============================================================================
-* Trace Low Equivalences
-*===========================================================================*)
-
-(* We might need two different definitions of trace low-equivalence
-* depending on the top-level security condition *)
-
-(* This is a straightforward definition of trace low-equivalence
-    Roughly, it says that 
-    t1 =L t2 <-> forall i, t1[i] =L t2[i].
-
-    This definition would be useful for a 
-    "possibilistic security condition". A possibilistic security condition
-    says that two executions look the same from the perspective of an observer
-    if all _possible behaviors_ look the same if they begin from initial states
-    that look the same to the observer.
-
-    Possibilistic security conditions say that
-    forall s1 s2 t1, 
-        (s1 =L s2 -> <c, s1> => t1),
-        exists t2, <c, s2> => t2 /\ t1 =L t2.
-
-    In other words there is some way to reach an execution trace
-    that looks the same beginning from the other state.
-    
-    Trapeze uses a possibilistic definition of security:
-    https://pdfs.semanticscholar.org/809b/f2702a765b9e7dba4624a1dbc53af11579db.pdf
-    See also:
-    https://www.cs.cornell.edu/andru/papers/csfw03.pdf
-
-    and discussion in PossibilisticNI.v
-*)
-
-Inductive trace_low_eq: @trace_low_eqT (state * (@labeled event)) :=
-    | NilEQ ell: trace_low_eq ell [] []
-    | AddBoth ell xs xe ys ye t1 t2:
-        trace_low_eq ell t1 t2 ->
-        event_low_eq ell xe ye ->
-        state_low_eq ell xs ys ->
-        trace_low_eq ell ((xs, xe)::t1) ((ys, ye)::t2).
-
-
-(* An alternative way of specifying security for
-   concurrent systems is observational determinism, which says
-   that for any two executions that begin from low-equivalent
-   initial states, the actual observed behaviors 
-   (by contrast to possibly observed behaviors)
-   _always_ look the same.
-
-    This looks like:
-    forall s1 s2 t1 t2,
-        (s1 =L s2) /\
-        (step_multi s1) => t1 /\
-        (step_multi s2) => t2 ->
-            t1 =L t2.
-
-    If we write this top-level theorem using the straightforward
-    definition of trace low-equivalence from above, the security condition
-    would rule out *some* timing channels that we know our system does not
-    prevent (so the security condition would not work). 
-
-    The straightforward security condition would rule out the case where:
-    - The observer is L
-    - There is label L' s.t. not (L' flowsTo L)
-    - A node called Other with Label L' takes more state transitions in one execution to
-    perform some computation than in the other.
-
-    While the "Other" node is executing, it can only affect parts of the system
-    labeled L' (or higher), so for this part of a single execution, it will
-    look like a sequence where ... si =L si+1 =L si+2 ... . In other words, the
-    sub-sequence is low-equivalent. If the observer really can't measure time,
-    two sequences that differ just in the number of transitions by "Other"
-    really do look the same.
-
-    This definition of trace low-equivalence rules this out by collapsing
-    adjacent low-equivalent states (called "high stutter") in the traces.
-*)
-Inductive stut_trace_low_eq: level -> trace -> trace -> Prop :=
-    | SNilEQ ell: stut_trace_low_eq ell [] []
-    | SAddBoth ell xs xe ys ye t1 t2:
-        stut_trace_low_eq ell t1 t2 ->
-        event_low_eq ell xe ye ->
-        state_low_eq ell xs ys ->
-        stut_trace_low_eq ell ((xs, xe)::t1) ((ys, ye)::t2)
-    | SAddEqR ell xs xe ys ye t1 t2:
-        stut_trace_low_eq ell t1 ((ys, ye)::t2) ->
-        event_low_eq ell xe ye ->
-        state_low_eq ell xs ys ->
-        stut_trace_low_eq ell t1 ((xs, xe)::(ys, ye)::t2)
-    | SAddEqL ell xs xe ys ye t1 t2:
-        stut_trace_low_eq ell ((ys, ye)::t1) t2 ->
-        event_low_eq ell xe ye ->
-        state_low_eq ell xs ys ->
-        stut_trace_low_eq ell ((xs, xe)::(ys, ye)::t1) t2.
