experimental/ni_coq/vfiles/EscapeHatchCondition_def.v
@@ -1,0 +1,32 @@
+Require Import Coq.Lists.List.
+Import ListNotations.
+From OakIFC Require Import
+    Lattice
+    Parameters
+    ModelTypes
+    State
+    Events
+    LowEquivalences
+    ModelTypes
+    TraceLowEq.
+
+
+Definition eh_t := @trace (state * down_l * event_l).
+Definition is_init(t: eh_t) := length t = 1.
+
+Definition eh_trace_low_eq: @trace_low_eqT (state * down_l *event_l) := 
+    @trace_low_eq_down state_low_eq down_low_eq event_low_eq.
+
+Definition conjecture_escape_hatch
+    (sem: @trace_semanticsT (state * down_l * event_l)) :=
+    forall ell t1_init t2_init dt1 dt2 t1n,
+    (eh_trace_low_eq ell t1_init t2_init) /\
+    (down_list_low_eq ell dt1 dt2) /\
+    (is_init t1_init) /\
+    (is_init t2_init) /\
+    (dt1 = (extract_downgrade_trace t1n)) /\
+    (sem t1_init t1n) ->
+    (exists t2n,
+        (sem t2_init t2n) /\
+        (eh_trace_low_eq ell t1n t2n) /\
+        (dt2 = (extract_downgrade_trace t2n))).
