experimental/ni_coq/vfiles/EvAugSemanticsDwn.v
@@ -1,0 +1,114 @@
+Require Import Coq.Sets.Ensembles.
+Require Import List.
+From OakIFC Require Import
+    Lattice
+    Parameters
+    GenericMap
+    ModelSemUtils
+    RuntimeModel
+    State
+    Events.
+Import ListNotations.
+
+From RecordUpdate Require Import RecordSet.
+Import RecordSetNotations.
+
+Local Open Scope map_scope.
+Local Open Scope ev_notation.
+
+Inductive step_node_ev (id: node_id): call -> state -> down_l ->
+        state -> event_l -> Prop :=
+    | SWriteChanEv s nlbl han msg s':
+        (s.(nodes) .[?id]).(lbl) = nlbl ->
+        step_node id (WriteChannel han msg) s s' ->
+        step_node_ev id (WriteChannel han msg) s (ell DWN nil)
+            s' (nlbl ---> msg)
+        (* The notations used for events on this last line and others
+        is in Events.v *)
+    | SWriteChanDwnEv s nlbl han msg s' ell':
+        (s.(nodes) .[?id]).(lbl) = nlbl ->
+        step_node id (WriteChannel han msg ell') s s' ->
+        step_node_ev id (WriteChannel han msg ell') s (msg DWN nlbl |--> ell')
+            s' (nlbl ---> msg)
+    | SReadChanEv s nlbl han chan msg s':
+        (s.(nodes) .[?id]).(lbl) = nlbl ->
+        step_node id (ReadChannel han) s s' ->
+        msg_is_head chan msg ->
+        step_node_ev id (ReadChannel han) s (ell DWN nil)
+            s' (nlbl <--- msg)
+    | SCreateChanEv s nlbl clbl s':
+        (* It seems clear that no event is needed since nodes only observe
+        * contents of channels indirectly via reads *)
+        (s.(nodes) .[?id]).(lbl) = nlbl ->
+        step_node id (CreateChannel clbl) s s' ->
+        step_node_ev id (CreateChannel clbl) s (ell DWN nil)
+            s' (nlbl --- )
+    | SCreateNodeEv s nlbl new_lbl h s':
+        (s.(nodes) .[?id]).(lbl) = nlbl ->
+        step_node id (CreateNode new_lbl h) s s' ->
+        step_node_ev id (CreateNode new_lbl h) s (ell DWN nil)
+            s' ( -- nlbl -- )
+    | SWaitOnChannelsEv s hs nlbl s':
+        (s.(nodes) .[?id]).(lbl) = nlbl ->
+        step_node id (WaitOnChannels hs) s s' ->
+        step_node_ev id (WaitOnChannels hs) s (ell DWN nil)
+            s' (nlbl ---)
+    | SChannelCloseEv s han nlbl s':
+        (s.(nodes) .[?id]).(lbl) = nlbl ->
+        step_node id (ChannelClose han) s s' ->
+        step_node_ev id (ChannelClose han) s (ell DWN nil)
+            s' (nlbl ---)
+    | SNodeLabelReadEv s nlbl s':
+        (s.(nodes) .[?id]).(lbl) = nlbl ->
+        step_node id NodeLabelRead s s' ->
+        step_node_ev id NodeLabelRead s (ell DWN nil)
+            s' (nlbl <--L nlbl)
+    | SChannelLabelReadEv s han nlbl clbl s':
+        (s.(nodes) .[?id]).(lbl) = nlbl ->
+        (s.(chans) .[?han]).(lbl) = clbl ->
+        step_node id (ChannelLabelRead han) s s' ->
+        step_node_ev id (ChannelLabelRead han) s (ell DWN nil)
+            s' (nlbl <--L clbl)
+    | SInternalEv s nlbl s':
+        (s.(nodes) .[?id]).(lbl) = nlbl ->
+        step_node id Internal s s' ->
+        step_node_ev id Internal s (ell DWN nil)
+            s' (nlbl ---).
+
+Inductive step_system_ev: state -> state -> event_l -> Prop :=
+    | SytsemEvSkip s ell: step_system_ev s s (ell ---) 
+    | SystemEvStepNode id n c c' s s' e:
+        (s.(nodes).[?id]).(obj) = Some n ->
+        n.(ncall) = c ->
+        step_node_ev id c s s' e ->
+        let s'' := (s_set_call s' id c') in
+            (* Here c' is an arbitrary command. The next ABI call
+            that the node makes after the one executed here is an arbitrary one
+            of that node's choosing *)
+        step_system_ev s s'' e.
+
+Definition trace := list (state * event_l).
+
+(* This is used for state/event pairs in EvAug. 
+* The type is slightly awkward now post refactor *)
+Definition head_st (t: trace) :=
+    match t with 
+        | nil => None
+        | (s', _)::_ => Some s'
+    end.
+
+Inductive step_system_ev_t: trace -> trace -> Prop :=
+    | StepTrace t s s' e:
+        head_st t = Some s -> 
+        step_system_ev s s' e ->
+        step_system_ev_t t ((s', e) :: t).
+
+Inductive step_system_ev_multi: trace -> trace -> Prop :=
+    | multi_system_ev_refl t t':
+        step_system_ev_t t t' ->
+        step_system_ev_multi t t'
+    | multi_system_ev_tran t1 t2 t3:
+        step_system_ev_t t2 t3 ->
+        step_system_ev_multi t1 t2 ->
+        step_system_ev_multi t1 t3.
+
