experimental/ni_coq/vfiles/RuntimeModelDwn.v
@@ -1,0 +1,203 @@
+Require Import List.
+Import ListNotations.
+Require Import Coq.Sets.Ensembles.
+From OakIFC Require Import
+    Lattice
+    Parameters
+    GenericMap
+    State
+    ModelSemUtils.
+
+(* This file is the top-level model of the Oak runtime *)
+
+(* RecordUpdate is a conveninece feature that provides functional updates for
+* records with notation: https://github.com/tchajed/coq-record-update *)
+(* To work with record updates from this library in proofs "unfold set" quickly
+* changes goals back to normal Coq built-in record updates *)
+From RecordUpdate Require Import RecordSet.
+Import RecordSetNotations.
+Local Open Scope map_scope.
+
+
+(* Ensembles don't have implicit type params and these lines fix that *)
+Arguments Ensembles.In {U}.
+Arguments Ensembles.Add {U}.
+Arguments Ensembles.Subtract {U}.
+Arguments Ensembles.Singleton {U}.
+Arguments Ensembles.Union {U}.
+Arguments Ensembles.Setminus {U}.
+Arguments Ensembles.Included {U}.
+
+(*============================================================================
+* Single Call Semantics
+============================================================================*)
+
+(* step for a single node (which can be thought of as a thread) executing
+* a particular call *)
+(* It might be akwkard looking that the call of a node is a part of the object,
+but that there is no premise checking that this call is really the one used
+in the relation. This is checked in the global transition relation just below.
+*)
+Inductive step_node (id: node_id): call -> state -> state -> Prop :=
+    | SWriteChan s n nlbl han clbl msg:
+        (s.(nodes).[?id]) = Labeled node (Some n) nlbl ->
+            (* caller is a real node with label nlbl *)
+        (s.(chans).[? han]).(lbl) = clbl ->
+            (* the handle has label clbl, though the call does not
+            check whether or not a channel is allocated to the handle
+            to avoid leaks (it can be Some or None) *)
+        In n.(write_handles) han ->     (* caller has write handle *)
+        nlbl <<L clbl ->     (* label of caller flowsTo label of ch*)
+        Included msg.(rhs) n.(read_handles) ->
+            (* caller has read handles it is sending *)
+        Included msg.(whs) n.(write_handles) ->
+            (* caller has write handles it is sending *)
+        let n' := node_del_rhans msg.(rhs) n in 
+            (* remove the read handles from the sender because read
+            * handles (but not write handles) are linear *)
+        let s0 := state_upd_node id n' s in
+            (* NOTE: throwing an error if the channel is not valid would cause
+            a leak. It might be possible to still prove NI if the write call
+            always proceeds regarldess of validity but only pushes to the 
+            validity, but only append the message if *)
+        step_node id (WriteChannel han msg) s 
+            (state_chan_append_labeled han msg (state_upd_node id n' s))
+    | SWriteChanDwn s n nlbl han clbl msg ell':
+        (s.(nodes).[? id]) = Labeled node (Some n) nlbl ->
+            (* caller is a real node with label nlbl *)
+        (s.(chans).[? han]).(lbl) = clbl ->
+            (* the handle has label clbl, though the call does not
+            check whether or not a channel is allocated to the handle
+            to avoid leaks (it can be Some or None) *)
+        In n.(write_handles) han ->     (* caller has write handle *)
+        Included msg.(rhs) n.(read_handles) ->
+            (* caller has read handles it is sending *)
+        Included msg.(whs) n.(write_handles) ->
+            (* caller has write handles it is sending *)
+        let n' := node_del_rhans msg.(rhs) n in 
+            (* remove the read handles from the sender because read
+            * handles (but not write handles) are linear *)
+        let s0 := state_upd_node id n' s in
+            (* NOTE: throwing an error if the channel is not valid would cause
+            a leak. It might be possible to still prove NI if the write call
+            always proceeds regarldess of validity but only pushes to the 
+            validity, but only append the message if *)
+        step_node id (WriteChannelDown han msg ell') s 
+            (state_chan_append_labeled han msg (state_upd_node id n' s))
+    | SReadChan s n nlbl han ch clbl msg:
+        (s.(nodes).[?id]) = Labeled node (Some n) nlbl ->
+            (* caller is a real node with label nlbl *)
+        (s.(chans).[?han]) = Labeled channel (Some ch) clbl ->  
+            (* handle points to real channel ch  with label clbl*)
+        In n.(read_handles) han ->   (* caller has read handle *)
+            (* A channel read happens only when there is a message
+            available in the channel. TODO, re-check what really happens
+            when a message is not available, and possibly improve the model.
+            E.g., if an error is thrown, execute an error continuation instead
+            of the usual one if an error is _not_ thrown.
+            *)
+        (msg_is_head ch msg) ->
+        channel_valid s han ->
+            (* the channel being read is not closed *)
+        clbl <<L nlbl ->
+            (* label of channel flowsTo label of caller. 
+                checks that reading the message is safe
+             *)
+        nlbl <<L clbl -> 
+            (* label of caller flowsTo label of ch. This check is less intuitive than the above.
+            However, reads are destructive because the channel is popped, so the calling node
+            is effectively doing a write to the channel. Any node that does a subsequent read
+            can detect whether or not the channel has been read because its contents may have 
+            been changed. This check rules out this more subtle leak *)
+        let n' := node_get_hans n msg in
+            (* node gets handles from channel *)
+        let ch' := chan_pop ch in
+            (* pop the message, clear the read/write handles in ch *)
+        step_node id (ReadChannel han) s
+            (state_upd_chan han ch' (state_upd_node id n' s))
+    | SCreateChan s n nlbl h clbl:
+        (s.(nodes).[?id]) = Labeled node (Some n) nlbl ->
+            (* caller is a real node with label nlbl *)
+        fresh_han s h ->
+            (* the target handle is not in use *)
+        nlbl = bot ->
+            (* only public/trusted nodes can create channels, for now *)
+            let s0 := (state_upd_chan_labeled h {|
+                obj := new_chan; lbl := clbl;
+            |} s) in
+            let s1 := state_upd_node id (node_add_rhan h n) s0 in
+            let s' := state_upd_node id (node_add_whan h n) s1 in
+            step_node id (CreateChannel clbl) s s'
+    | SCreateNode s n nlbl new_id new_lbl h:
+        (s.(nodes).[?id]) = Labeled node (Some n) nlbl ->
+            (* caller is a real node with label nlbl *)
+        fresh_nid s id ->
+            (* target nid is not in use *)
+        nlbl = bot ->
+            (* only public/trusted nodes can create nodes for now *)
+            (* create new node with read handle *)
+        let s0 := (state_upd_node_labeled new_id {|
+                obj := Some {|
+                    read_handles := (Singleton h);
+                    write_handles := Empty_set handle;
+                    ncall := Internal;
+                |};
+                lbl := new_lbl;
+            |} s) in
+        let s' := state_upd_node id (node_add_rhan h n) s0 in
+        step_node id (CreateNode new_lbl h) s s'
+    | SWaitOnChannels s n hs h ms nlbl clbl:
+        (s.(nodes).[?id]) = Labeled node (Some n) nlbl ->
+            (* caller is a real node with label nlbl *)
+        In hs h->
+            (* there is some handle h in the list of handles s.t. ... *)
+        s.(chans).[?h] = Labeled channel (Some (Chan ValidChannel ms)) clbl ->
+            (* It points to a valid channel s.t. ... *)
+        length ms > 0  -> (* it has some pending message and ... *)
+        clbl <<L nlbl -> (* its label flows to the label of the node *)
+            (* an alternative way to do this would be to check that the
+            the labels of all the channels in the list flowTo the label
+            of the node before blocking. This specification is implied
+            by that other one. *)
+        step_node id (WaitOnChannels hs) s s
+        (*
+            This specification says that we can't step out of a
+            WaitOnChannels until there is a non-empty channel in the list.
+            A better model might be one that:
+                - marks the node as blocked if this is not true
+                - in the global scheduler: only un-blocked nodes get scheduled
+        *)
+    | SChannelClose s n ch han nlbl clbl: 
+        (s.(nodes).[?id]) = Labeled node (Some n) nlbl ->
+            (* caller is a real node with label nlbl *)
+        (s.(chans).[?han]).(lbl) = clbl ->
+            (* handle has label clbl *)
+        nlbl <<L clbl ->
+        step_node id (ChannelClose han) s 
+            (state_upd_chan han (chan_close ch) s)
+    | SNodeLabelRead s:
+        step_node id NodeLabelRead s s
+    | SChannelLabelRead s han:
+        step_node id (ChannelLabelRead han) s s
+    | SInternal s: 
+        step_node id Internal s s.
+
+(* step for the full system which (non-deterministically) picks a thread to
+* execute. This is needed in addition to step_node, because
+we should show that regardless of the thread scheduling, there are no information
+leaks. *)
+(* To be general and language agnostic, computation of code within nodes other
+than the ABI calls is modeled as simply returning an arbitrary continuation 
+(c') of the node's choosing (for any call). *)
+(* Errors might later be modeled by choosing a different continuation based
+on whether or not a call was successful, in this case, the resulting
+continuation likely needs to be moved into the local transition relation *)
+
+Inductive step_system: state -> state -> Prop :=
+    (* possibly also a termination case *)
+    | SystemSkip s: step_system s s
+    | SystemStepNode id n c c' s s':
+        (s.(nodes) .[?id]).(obj) = Some n ->
+        n.(ncall) = c ->
+        step_node id c s s' ->
+        step_system s (s_set_call s id c').
